FOF_Simplify.thy
@@ -1,0 +1,159 @@
+theory FOF_Simplify
+  imports Main FOF_Base
+begin
+
+lemma eval_formula_Not_Not: "eval_formula (Not (Not f)) vI fI pI = eval_formula f vI fI pI"
+  by simp
+
+lemma eval_formula_simp_formula_Not_equiv:
+  assumes IH: "eval_formula (simp_formula \<phi>) vI fI pI = eval_formula \<phi> vI fI pI"
+  shows "eval_formula (simp_formula (Not \<phi>)) vI fI pI = eval_formula (Not \<phi>) vI fI pI"
+proof (cases "simp_formula \<phi>")
+  case (Pred p args)
+  have "eval_formula (simp_formula (Not \<phi>)) vI fI pI = eval_formula (Not (Pred p args)) vI fI pI"
+    using simp_formula.simps `simp_formula \<phi> = (Pred p args)`
+    by simp
+  also have "... = (\<not>(eval_formula (Pred p args) vI fI pI))"
+    using eval_formula.simps
+    by simp
+  also have "... = (\<not>(eval_formula \<phi>) vI fI pI)"
+    using `simp_formula \<phi> = (Pred p args)` IH
+    by simp
+  also have "... = eval_formula (Not \<phi>) vI fI pI"
+    using eval_formula.simps
+    by simp
+  finally show ?thesis .
+next
+  case (And f1 f2)
+  have "eval_formula (simp_formula (Not \<phi>)) vI fI pI = eval_formula (Not (And f1 f2)) vI fI pI"
+    using simp_formula.simps `simp_formula \<phi> = (And f1 f2)` 
+    by simp
+  also have "... = (\<not>(eval_formula (And f1 f2) vI fI pI))"
+    using eval_formula.simps
+    by simp
+  also have "... = eval_formula (Not \<phi>) vI fI pI"
+    using `simp_formula \<phi> = (And f1 f2)` IH eval_formula.simps
+    by simp
+  finally show ?thesis .
+next
+  case (Or f1 f2)
+  have "eval_formula (simp_formula (Not \<phi>)) vI fI pI = eval_formula (Not (Or f1 f2)) vI fI pI"
+    using simp_formula.simps `simp_formula \<phi> = (Or f1 f2)` 
+    by simp
+  also have "... = (\<not>(eval_formula (Or f1 f2) vI fI pI))"
+    using eval_formula.simps
+    by simp
+  also have "... = eval_formula (Not \<phi>) vI fI pI"
+    using `simp_formula \<phi> = (Or f1 f2)` IH eval_formula.simps
+    by simp
+  finally show ?thesis .  
+next
+  case (Not f)
+  have "eval_formula (simp_formula (Not \<phi>)) vI fI pI = eval_formula f vI fI pI"
+    using simp_formula.simps `simp_formula \<phi> = (Not f)` eval_formula_Not_Not
+    by simp
+  also have "... = (\<not>(\<not>(eval_formula f vI fI pI)))"
+    using eval_formula_Not_Not
+    by simp
+  also have "... = (\<not>(eval_formula \<phi> vI fI pI))"
+    using eval_formula.simps `simp_formula \<phi> = (Not f)` IH
+    by simp
+  also have "... = eval_formula (Not \<phi>) vI fI pI"
+    using eval_formula.simps
+    by simp 
+  finally show ?thesis .
+next
+  case (Equal t1 t2)
+  have "eval_formula (simp_formula (Not \<phi>)) vI fI pI = eval_formula (Not (Equal t1 t2)) vI fI pI"
+    using simp_formula.simps `simp_formula \<phi> = (Equal t1 t2)`
+    by simp
+  also have "... = (\<not>(eval_formula (Equal t1 t2) vI fI pI))"
+    using eval_formula.simps
+    by simp
+  also have "... = eval_formula (Not \<phi>) vI fI pI"
+    using `simp_formula \<phi> = (Equal t1 t2)` IH eval_formula.simps
+    by simp
+  finally show ?thesis .
+next
+  case (Forall v f)
+  have "eval_formula (simp_formula (Not \<phi>)) vI fI pI = eval_formula (Not (Forall v f)) vI fI pI"
+    using simp_formula.simps `simp_formula \<phi> = (Forall v f)`
+    by simp
+  also have "... = (\<not>(eval_formula (Forall v f) vI fI pI))"
+    using eval_formula.simps
+    by simp
+  also have "... = eval_formula (Not \<phi>) vI fI pI"
+    using `simp_formula \<phi> = (Forall v f)` IH eval_formula.simps
+    by simp
+  finally show ?thesis .
+next
+  case (Exists v f)
+  have "eval_formula (simp_formula (Not \<phi>)) vI fI pI = eval_formula (Not (Exists v f)) vI fI pI"
+    using simp_formula.simps `simp_formula \<phi> = (Exists v f)`
+    by simp
+  also have "... = (\<not>(eval_formula (Exists v f) vI fI pI))"
+    using eval_formula.simps
+    by simp
+  also have "... = eval_formula (Not \<phi>) vI fI pI"
+    using `simp_formula \<phi> = (Exists v f)` IH eval_formula.simps
+    by simp
+  finally show ?thesis .
+next
+  case T
+  have "eval_formula (simp_formula (Not \<phi>)) vI fI pI = False"
+    using simp_formula.simps `simp_formula \<phi> = T` eval_formula.simps
+    by simp
+  also have "... = (\<not>(eval_formula T vI fI pI))"
+    using eval_formula.simps
+    by simp
+  also have "... = eval_formula (Not \<phi>) vI fI pI"
+    using `simp_formula \<phi> = T` IH eval_formula.simps
+    by simp
+  finally show ?thesis .
+next
+  case F
+  have "eval_formula (simp_formula (Not \<phi>)) vI fI pI = True"
+    using simp_formula.simps `simp_formula \<phi> = F` eval_formula.simps
+    by simp
+  also have "... = (\<not>(eval_formula F vI fI pI))"
+    using eval_formula.simps
+    by simp
+  also have "... = eval_formula (Not \<phi>) vI fI pI"
+    using `simp_formula \<phi> = F` IH eval_formula.simps
+    by simp  
+  finally show ?thesis .
+qed
+
+(*
+theorem eval_formula_simp_formula_equiv_eval_formula: "eval_formula (simp_formula \<phi>) vI fI pI = eval_formula \<phi> vI fI pI"
+proof (induction \<phi> rule: simp_formula.induct)
+  case (1 p args)
+  then show ?case by simp
+next
+  case (2 f1 f2)
+  then show ?case sorry
+next
+  case (3 f1 f2)
+  then show ?case sorry
+next
+  case (4 f)
+  then show ?case by (rule eval_formula_simp_formula_Not_equiv)
+next
+  case (5 t1 t2)
+  then show ?case by simp
+next
+  case (6 v f)
+  then show ?case sorry
+next
+  case (7 v f)
+  then show ?case sorry
+next
+  case 8
+  then show ?case by simp
+next
+  case 9
+  then show ?case by simp
+qed
+*)
+
+end
